flex/src/FlexTLS.Message.ServerHelloDone.fst
@@ -3,7 +3,7 @@
 module FlexTLS.Message.ServerHelloDone
 
 
-open Platform.Log
+open Log
 open Platform.Bytes
 open Platform.Error
 
@@ -15,13 +15,16 @@ open FlexTLS.Handshake
 
 
 
+/// Access the log
+let log = Log.retrieve "FlexTLS.Log.General"
+
 /// <summary>
 /// Receive a ServerHelloDone message from the network stream
 /// </summary>
 /// <param name="st"> State of the current Handshake </param>
 /// <returns> Updated state * FServerHelloDone message record </returns>
 let receive (st:state) : state * FServerHelloDone =
-  Log.logInfo("# SERVER HELLO DONE : FlexServerHelloDone.receive");
+  Log.write log Info "TLS Message" ("# SERVER HELLO DONE : FlexServerHelloDone.receive");
   let st,hstype,payload,to_log = FlexHandshake.receive(st) in
   match hstype with
   | HT_server_hello_done  ->
@@ -29,7 +32,7 @@ let receive (st:state) : state * FServerHelloDone =
       failwith (perror __SOURCE_FILE__ __LINE__ "payload has not length zero")
     else
       let fshd: FServerHelloDone = {payload = to_log} in
-      Log.logDebug(sprintf "--- Payload : %s" (Bytes.hexString(payload)));
+      Log.write log Debug "" (sprintf "--- Payload : %s" (Bytes.hexString(payload)));
       st,fshd
   | _ -> failwith (perror __SOURCE_FILE__ __LINE__ (sprintf "Unexpected handshake type: %A" hstype))
 
@@ -50,7 +53,7 @@ let prepare () : FServerHelloDone =
 /// <param name="fp"> Optional fragmentation policy at the record level </param>
 /// <returns> Updated state * FServerHelloDone message record </returns>
 let send (st:state) (*?*)(fp:fragmentationPolicy) : state * FServerHelloDone =
-  Log.logInfo("# SERVER HELLO DONE : FlexServerHelloDone.send");
+  Log.write log Info "TLS Message" ("# SERVER HELLO DONE : FlexServerHelloDone.send");
   //  let fp = defaultArg fp FlexConstants.defaultFragmentationPolicy in
   let fshd = FlexServerHelloDone.prepare() in
   let st = FlexHandshake.send(st,fshd.payload,fp) in
