flex/src/FlexTLS.Types.fst
@@ -202,7 +202,7 @@ type FServerHello = {
   /// <summary> Server random bytes </summary>
   rand: bytes;
   /// <summary> Session identifier. A non-empty byte array indicates that the server accepted resumption </summary>
-  sid: option<bytes>;
+  sid: option bytes;
   /// <summary> Ciphersuite selected by the server </summary>
   ciphersuite: option cipherSuiteName;
   /// <summary> Compression selected by the server </summary>
